semantics/vyperTypeCallGraphScript.sml
@@ -1,0 +1,182 @@
+(*
+ * Executable internal-call graph analysis for checked Vyper contracts.
+ *
+ * TOP-LEVEL:
+ * - int_calls_expr / int_calls_stmt: syntactic internal-call extraction
+ * - contract_call_edges: whole-contract call graph
+ * - contract_call_graph_acyclic: bounded executable cycle check
+ *)
+
+Theory vyperTypeCallGraph
+Ancestors
+  list rich_list vyperAST
+Libs
+  cv_transLib
+
+(* ===== Internal calls in expressions and assignment targets ===== *)
+
+Definition int_calls_expr_def:
+  int_calls_expr (Name _ _) = [] /\
+  int_calls_expr (TopLevelName _ _) = [] /\
+  int_calls_expr (FlagMember _ _ _) = [] /\
+  int_calls_expr (IfExp _ c x y) =
+    int_calls_expr c ++ int_calls_expr x ++ int_calls_expr y /\
+  int_calls_expr (Literal _ _) = [] /\
+  int_calls_expr (StructLit _ _ kes) = int_calls_named_exprs kes /\
+  int_calls_expr (Subscript _ x y) = int_calls_expr x ++ int_calls_expr y /\
+  int_calls_expr (Attribute _ x _) = int_calls_expr x /\
+  int_calls_expr (Builtin _ _ es) = int_calls_exprs es /\
+  int_calls_expr (TypeBuiltin _ _ _ es) = int_calls_exprs es /\
+  int_calls_expr (Pop _ tgt) = int_calls_target tgt /\
+  int_calls_expr (Call _ (IntCall callee) es _) =
+    callee :: int_calls_exprs es /\
+  int_calls_expr (Call _ (ExtCall _ _) es default_ret) =
+    int_calls_exprs es ++ int_calls_opt default_ret /\
+  int_calls_expr (Call _ _ es _) = int_calls_exprs es /\
+
+  int_calls_target (NameTarget _) = [] /\
+  int_calls_target (TopLevelNameTarget _) = [] /\
+  int_calls_target (SubscriptTarget tgt e) =
+    int_calls_target tgt ++ int_calls_expr e /\
+  int_calls_target (AttributeTarget tgt _) = int_calls_target tgt /\
+
+  int_calls_exprs [] = [] /\
+  int_calls_exprs (e::es) = int_calls_expr e ++ int_calls_exprs es /\
+
+  int_calls_opt NONE = [] /\
+  int_calls_opt (SOME e) = int_calls_expr e /\
+
+  int_calls_named_exprs [] = [] /\
+  int_calls_named_exprs ((_,e)::kes) =
+    int_calls_expr e ++ int_calls_named_exprs kes
+Termination
+  WF_REL_TAC `measure (\(x : expr + base_assignment_target + expr list +
+                                      expr option + (identifier # expr) list).
+    case x of
+    | INL e => expr_size e
+    | INR (INL tgt) => base_assignment_target_size tgt
+    | INR (INR (INL es)) => expr4_size es
+    | INR (INR (INR (INL opt))) => expr3_size opt
+    | INR (INR (INR (INR kes))) => expr1_size kes)` >>
+  simp[expr_size_def] >>
+  qsuff_tac
+    `(!es. expr4_size es = list_size expr_size es) /\
+     (!opt. expr3_size opt = option_size expr_size opt) /\
+     (!kes. expr1_size kes =
+       list_size (pair_size (list_size char_size) expr_size) kes)`
+  >- (strip_tac >> asm_rewrite_tac[] >> DECIDE_TAC) >>
+  rpt conj_tac >>
+  TRY (Induct >> simp[expr_size_def, listTheory.list_size_def,
+        basicSizeTheory.pair_size_def]) >>
+  Cases >> simp[expr_size_def, basicSizeTheory.option_size_def]
+End
+
+(* ===== Internal calls in statements ===== *)
+
+Definition int_calls_atarget_def:
+  int_calls_atarget (BaseTarget tgt) = int_calls_target tgt /\
+  int_calls_atarget (TupleTarget tgts) = int_calls_atargets tgts /\
+  int_calls_atargets [] = [] /\
+  int_calls_atargets (t::ts) = int_calls_atarget t ++ int_calls_atargets ts
+Termination
+  WF_REL_TAC `measure (\x. case x of
+    | INL tgt => assignment_target_size tgt
+    | INR tgts => assignment_target1_size tgts)` >>
+  simp[]
+End
+
+Definition int_calls_iterator_def:
+  int_calls_iterator (Array e) = int_calls_expr e /\
+  int_calls_iterator (Range x y) = int_calls_expr x ++ int_calls_expr y
+End
+
+Definition int_calls_assert_reason_def:
+  int_calls_assert_reason AssertBare = [] /\
+  int_calls_assert_reason AssertUnreachable = [] /\
+  int_calls_assert_reason (AssertReason e) = int_calls_expr e
+End
+
+Definition int_calls_raise_reason_def:
+  int_calls_raise_reason RaiseBare = [] /\
+  int_calls_raise_reason RaiseUnreachable = [] /\
+  int_calls_raise_reason (RaiseReason e) = int_calls_expr e
+End
+
+Definition int_calls_stmt_def:
+  int_calls_stmt Pass = [] /\
+  int_calls_stmt Continue = [] /\
+  int_calls_stmt Break = [] /\
+  int_calls_stmt (Expr e) = int_calls_expr e /\
+  int_calls_stmt (For _ _ iter _ body) =
+    int_calls_iterator iter ++ int_calls_stmts body /\
+  int_calls_stmt (If e yes no) =
+    int_calls_expr e ++ int_calls_stmts yes ++ int_calls_stmts no /\
+  int_calls_stmt (Assert e reason) =
+    int_calls_expr e ++ int_calls_assert_reason reason /\
+  int_calls_stmt (Log _ es) = int_calls_exprs es /\
+  int_calls_stmt (Raise reason) = int_calls_raise_reason reason /\
+  int_calls_stmt (Return opt) = int_calls_opt opt /\
+  int_calls_stmt (Assign tgt e) = int_calls_atarget tgt ++ int_calls_expr e /\
+  int_calls_stmt (AugAssign _ tgt _ e) =
+    int_calls_target tgt ++ int_calls_expr e /\
+  int_calls_stmt (Append tgt e) = int_calls_target tgt ++ int_calls_expr e /\
+  int_calls_stmt (AnnAssign _ _ e) = int_calls_expr e /\
+
+  int_calls_stmts [] = [] /\
+  int_calls_stmts (s::ss) = int_calls_stmt s ++ int_calls_stmts ss
+Termination
+  WF_REL_TAC `measure (\x. case x of
+    | INL s => stmt_size s
+    | INR ss => list_size stmt_size ss)` >>
+  simp[]
+End
+
+(* ===== Contract graph construction ===== *)
+
+Definition function_int_calls_def:
+  function_int_calls dflts body = int_calls_exprs dflts ++ int_calls_stmts body
+End
+
+Definition toplevel_call_edges_def:
+  toplevel_call_edges src
+    (FunctionDecl _ _ _ _ fn _ dflts _ body) =
+      MAP (\callee. ((src,fn),callee)) (function_int_calls dflts body) /\
+  toplevel_call_edges _ _ = []
+End
+
+Definition module_call_edges_def:
+  module_call_edges (src,tls) = FLAT (MAP (toplevel_call_edges src) tls)
+End
+
+Definition contract_call_edges_def:
+  contract_call_edges mods = FLAT (MAP module_call_edges mods)
+End
+
+Definition contract_call_nodes_def:
+  contract_call_nodes mods =
+    nub (MAP FST (contract_call_edges mods) ++ MAP SND (contract_call_edges mods))
+End
+
+(* ===== Executable bounded reachability and acyclicity ===== *)
+
+Definition direct_callees_def:
+  direct_callees edges caller = MAP SND (FILTER (\edge. FST edge = caller) edges)
+End
+
+Definition reachable_nodes_def:
+  reachable_nodes edges 0 caller = nub (direct_callees edges caller) /\
+  reachable_nodes edges (SUC fuel) caller =
+    let reached = reachable_nodes edges fuel caller in
+      nub (reached ++ FLAT (MAP (direct_callees edges) reached))
+End
+
+Definition call_graph_acyclic_def:
+  call_graph_acyclic nodes edges <=>
+    EVERY (\node. ~MEM node (reachable_nodes edges (LENGTH nodes) node)) nodes
+End
+
+Definition contract_call_graph_acyclic_def:
+  contract_call_graph_acyclic mods <=>
+    call_graph_acyclic (contract_call_nodes mods) (contract_call_edges mods)
+End
+
